matching-logic/src/Theories/Nat_ProofSystem.v
@@ -107,7 +107,7 @@ Section nat.
     { set_solver. }
   Defined.
 
-  Theorem peano_induction X :
+  Theorem peano_induction_meta X :
     theory ⊢ patt_free_svar X ⊆ml 〚 Nat 〛 ->
     theory ⊢ Zero ∈ml patt_free_svar X ->
     theory ⊢ all Nat, (b0 ∈ml patt_free_svar X ---> Succ $ b0 ∈ml patt_free_svar X) ->
@@ -315,6 +315,125 @@ Section nat.
       + mlExact "ys".
     }
   Defined.
+
+  Theorem peano_induction X :
+    theory ⊢ patt_free_svar X ⊆ml 〚 Nat 〛 --->
+             Zero ∈ml patt_free_svar X --->
+             (all Nat, (b0 ∈ml patt_free_svar X ---> Succ $ b0 ∈ml patt_free_svar X))--->
+             all Nat, b0 ∈ml patt_free_svar X.
+  Proof.
+    toMLGoal.
+    { wf_auto2. }
+    mlIntro "H".
+    mlIntro "H1".
+    mlIntro "H2".
+
+    mlApplyMeta nat_subset_imp_in.
+    remember (evar_fresh []) as x.
+    pose proof membership_symbol_ceil_aux_aux_0 theory x ( patt_free_svar X) 
+                                         ltac:( unfold theory;set_solver) ltac:(wf_auto2) as H.
+   apply universal_generalization with (x:=x) in H.
+   2: try_solve_pile.
+   2: wf_auto2.
+   mlSimpl in H. simpl in H.
+   case_match. 2: congruence.
+   assert ( theory ⊢ (ex , Zero =ml b0) ). {
+     pose proof (hypothesis theory (ex Nat, Zero =ml b0) ltac:(wf_auto2)).
+     ospecialize* H1.
+     { unfold theory, named_axioms, theory_of_NamedAxioms. simpl.
+       apply elem_of_union_r. exists AxFun1. reflexivity.
+     }
+     use AnyReasoning in H1.
+     mlAdd H1 as "H".
+     mlDestructEx "H" as x. mlSimpl. cbn. mlDestructAnd "H".
+     mlExists x. mlAssumption.
+   }
+   use AnyReasoning in H.
+(*    epose proof conj_intro_meta _ _ _ _ _ _ H H1.
+   Unshelve.
+   2-3: wf_auto2. *)
+     mlSpecMeta H with Zero.
+     2:unfold theory;set_solver.
+     2:simpl;reflexivity.
+     mlSimpl in H.
+     simpl in H.
+     mlApplyMeta H in "H1".
+
+     Search patt_and patt_total.
+     unfold patt_forall_of_sort.
+     
+     Search patt_exists patt_total derives_using.
+    (* rephrase "H2" into a totality statement and use propagation of totality through conjuction  *)
+ Admitted.
+
+  Lemma floor_propagation_forall_1 :
+    forall Γ φ,
+      Definedness_Syntax.theory ⊆ Γ ->
+      well_formed (ex, φ) ->
+      Γ ⊢ (all , ⌊φ⌋) ---> ⌊all , φ⌋.
+  Proof.
+    intros Γ φ HΓ Hwf.
+    unfold patt_forall.
+    mlIntro "H". mlIntro "H0".
+    mlApplyMeta def_not_phi_impl_not_total_phi in "H0". 2: assumption.
+    pose proof (def_propagate_not Γ (ex, ! φ) HΓ ltac:(wf_auto2)) as H.
+    use AnyReasoning in H. mlAdd H as "H1".
+    mlDestructAnd "H1" as "H1_1" "H1_2".
+    mlApply "H0". mlApply "H1_1". mlClear "H1_1". mlClear "H1_2".
+    mlClear "H0".
+    mlIntro "H0".
+    mlApply "H". mlClear "H".
+    mlApplyMeta ceil_propagation_exists_1 in "H0". 2: assumption.
+    mlDestructEx "H0" as x. mlExists x. mlSimpl.
+    mlApplyMeta def_not_phi_impl_not_total_phi in "H0". 2: assumption.
+    mlAssumption.
+  Defined.
+
+  Lemma exists_exists_of_sort :
+    forall Γ φ s,
+      Definedness_Syntax.theory ⊆ Γ ->
+      well_formed (ex, φ) ->
+      well_formed s ->
+      Γ ⊢ (ex s, φ) ---> ex, φ.
+  Proof.
+    intros Γ φ s HΓ wf1 wf2.
+    mlIntro "H".
+    remember (fresh_evar (s $ φ)) as x.
+    mlDestructEx "H" as x. rewrite free_evars_nest_ex. solve_fresh.
+    mlExists x. mlSimpl. cbn. mlDestructAnd "H". mlExact "1".
+  Defined.
+
+  Lemma predicate_imp :
+    forall Γ φ ψ,
+      Definedness_Syntax.theory ⊆ Γ ->
+      well_formed φ ->
+      well_formed ψ ->
+      Γ ⊢ is_predicate φ --->
+          is_predicate ψ --->
+          is_predicate (φ ---> ψ).
+  Proof.
+    intros Γ φ ψ HΓ wf1 wf2.
+    mlIntro "H". mlIntro "H0".
+    unfold is_predicate. mlDestructOr "H"; mlDestructOr "H0".
+    all: mlRewriteBy "0" at 1; mlRewriteBy "1" at 1.
+    all: mlRewriteBy "0" at 1; mlRewriteBy "1" at 1.
+  Defined.
+
+  Lemma predicate_equiv :
+    forall Γ φ,
+      Definedness_Syntax.theory ⊆ Γ ->
+      well_formed φ ->
+      Γ ⊢ is_predicate φ ---> φ <---> ⌊φ⌋.
+  Proof.
+    
+  Defined.
+
+  Lemma patt_in_is_predicate :
+    forall Γ φ ψ,
+      Definedness_Syntax.theory ⊆ Γ ->
+      well_formed φ ->
+      well_formed ψ ->
+      Γ ⊢ is_functional φ ---> is_predicate ψ ---> is_predicate (φ ∈ml ψ)
 
 End nat.
 
